candle/cv_compute_whole_box_dim_taylor.ml
@@ -84,6 +84,33 @@ let candle_q_dim_whole_box_upper_def = new_definition
         (candle_q_center_environment_list boxes) pds)
       (candle_q_program_interval_matrix boxes pdds)`;;
 
+let candle_q_box_valid_list_def = define
+ `(candle_q_box_valid_list [] <=> T) /\
+  (candle_q_box_valid_list (CONS h t) <=>
+     candle_q_le (FST h) (SND h) /\ candle_q_box_valid_list t)`;;
+
+let candle_q_rows_width_def = define
+ `(candle_q_rows_width n
+     ([]:((candle_q_instruction list)list)list) <=> T) /\
+  (candle_q_rows_width n (CONS h t) <=>
+     LENGTH h = n /\ candle_q_rows_width n t)`;;
+
+let candle_q_dim_inputs_valid_def = new_definition
+ `candle_q_dim_inputs_valid
+    (pds:(candle_q_instruction list)list)
+    (pdds:((candle_q_instruction list)list)list)
+    (boxes:(((num#num)#num)#((num#num)#num))list) <=>
+    LENGTH pds = LENGTH boxes /\
+    LENGTH pdds = LENGTH boxes /\
+    candle_q_rows_width (LENGTH boxes) pdds`;;
+
+let candle_q_dim_whole_box_accept_def = new_definition
+ `candle_q_dim_whole_box_accept pf pds pdds boxes <=>
+    candle_q_dim_inputs_valid pds pdds boxes /\
+    candle_q_box_valid_list boxes /\
+    ~(candle_q_le candle_q_zero
+       (candle_q_dim_whole_box_upper pf pds pdds boxes))`;;
+
 (* cval encodings for program vectors/matrices and exact-rational vectors. *)
 
 let candle_cv_q_instruction_lists_def = define
@@ -176,6 +203,54 @@ let candle_cv_q_dim_whole_box_upper_def = new_definition
         (candle_cv_q_center_environment_list boxes) pds)
       (candle_cv_q_program_interval_matrix boxes pdds)`;;
 
+let candle_cv_list_length_def = define
+ `(candle_cv_list_length (Cexp_num n) = Cexp_num 0) /\
+  (candle_cv_list_length (Cexp_pair h t) =
+     Cexp_add (Cexp_num 1) (candle_cv_list_length t))`;;
+
+let candle_cv_q_box_valid_list_def = define
+ `(candle_cv_q_box_valid_list (Cexp_num n) = Cexp_num 1) /\
+  (candle_cv_q_box_valid_list (Cexp_pair h t) =
+     Cexp_if
+       (candle_cv_q_le (Cexp_fst h) (Cexp_snd h))
+       (candle_cv_q_box_valid_list t) (Cexp_num 0))`;;
+
+let candle_cv_q_rows_width_def = define
+ `(candle_cv_q_rows_width n (Cexp_num z) = Cexp_num 1) /\
+  (candle_cv_q_rows_width n (Cexp_pair h t) =
+     Cexp_if (Cexp_eq (candle_cv_list_length h) n)
+       (candle_cv_q_rows_width n t) (Cexp_num 0))`;;
+
+let candle_cv_q_dim_inputs_valid_def = new_definition
+ `candle_cv_q_dim_inputs_valid pds pdds boxes =
+    Cexp_if
+      (Cexp_eq (candle_cv_list_length pds)
+        (candle_cv_list_length boxes))
+      (Cexp_if
+        (Cexp_eq (candle_cv_list_length pdds)
+          (candle_cv_list_length boxes))
+        (candle_cv_q_rows_width (candle_cv_list_length boxes) pdds)
+        (Cexp_num 0))
+      (Cexp_num 0)`;;
+
+let candle_cv_q_dim_whole_box_finish_def = new_definition
+ `candle_cv_q_dim_whole_box_finish inputs_valid box_valid upper =
+    Cexp_pair
+      (Cexp_if inputs_valid
+        (Cexp_if box_valid
+          (Cexp_if (candle_cv_q_le candle_cv_q_zero upper)
+            (Cexp_num 0) (Cexp_num 1))
+          (Cexp_num 0))
+        (Cexp_num 0))
+      upper`;;
+
+let candle_cv_q_dim_whole_box_check_def = new_definition
+ `candle_cv_q_dim_whole_box_check pf pds pdds boxes =
+    candle_cv_q_dim_whole_box_finish
+      (candle_cv_q_dim_inputs_valid pds pdds boxes)
+      (candle_cv_q_box_valid_list boxes)
+      (candle_cv_q_dim_whole_box_upper pf pds pdds boxes)`;;
+
 let candle_cv_q_center_environment_list_compute = prove
  (`!boxes.
      candle_cv_q_center_environment_list boxes =
@@ -264,6 +339,49 @@ let candle_cv_q_weighted_rows_abs_upper_compute = prove
   REWRITE_TAC[candle_cv_q_weighted_rows_abs_upper_def;
               cexp_if_def; cexp_ispair_def; cexp_fst_def; cexp_snd_def]);;
 
+let candle_cv_list_length_compute = prove
+ (`!items.
+     candle_cv_list_length items =
+     Cexp_if (Cexp_ispair items)
+       (Cexp_add (Cexp_num 1)
+         (candle_cv_list_length (Cexp_snd items)))
+       (Cexp_num 0)`,
+  GEN_TAC THEN
+  STRUCT_CASES_TAC (SPEC `items:cval` (cases "cval")) THEN
+  REWRITE_TAC[candle_cv_list_length_def;
+              cexp_if_def; cexp_ispair_def; cexp_snd_def]);;
+
+let candle_cv_q_box_valid_list_compute = prove
+ (`!boxes.
+     candle_cv_q_box_valid_list boxes =
+     Cexp_if (Cexp_ispair boxes)
+       (Cexp_if
+         (candle_cv_q_le
+           (Cexp_fst (Cexp_fst boxes))
+           (Cexp_snd (Cexp_fst boxes)))
+         (candle_cv_q_box_valid_list (Cexp_snd boxes))
+         (Cexp_num 0))
+       (Cexp_num 1)`,
+  GEN_TAC THEN
+  STRUCT_CASES_TAC (SPEC `boxes:cval` (cases "cval")) THEN
+  REWRITE_TAC[candle_cv_q_box_valid_list_def;
+              cexp_if_def; cexp_ispair_def; cexp_fst_def; cexp_snd_def]);;
+
+let candle_cv_q_rows_width_compute = prove
+ (`!n row_lists.
+     candle_cv_q_rows_width n row_lists =
+     Cexp_if (Cexp_ispair row_lists)
+       (Cexp_if
+         (Cexp_eq
+           (candle_cv_list_length (Cexp_fst row_lists)) n)
+         (candle_cv_q_rows_width n (Cexp_snd row_lists))
+         (Cexp_num 0))
+       (Cexp_num 1)`,
+  REPEAT GEN_TAC THEN
+  STRUCT_CASES_TAC (SPEC `row_lists:cval` (cases "cval")) THEN
+  REWRITE_TAC[candle_cv_q_rows_width_def;
+              cexp_if_def; cexp_ispair_def; cexp_fst_def; cexp_snd_def]);;
+
 let candle_cv_q_dim_whole_box_compute_eqs =
   candle_cv_q_interval_program_compute_eqs @
   map SPEC_ALL
@@ -280,8 +398,14 @@ let candle_cv_q_dim_whole_box_compute_eqs =
     candle_cv_q_program_interval_matrix_compute;
     candle_cv_q_dot_abs_upper_compute;
     candle_cv_q_weighted_rows_abs_upper_compute;
+    candle_cv_list_length_compute;
+    candle_cv_q_box_valid_list_compute;
+    candle_cv_q_rows_width_compute;
+    candle_cv_q_dim_inputs_valid_def;
+    candle_cv_q_dim_whole_box_finish_def;
     candle_cv_q_dim_taylor_upper_def;
-    candle_cv_q_dim_whole_box_upper_def];;
+    candle_cv_q_dim_whole_box_upper_def;
+    candle_cv_q_dim_whole_box_check_def];;
 
 (* Representation theorems. *)
 
@@ -408,5 +532,149 @@ let candle_cv_q_dim_whole_box_upper_correct = prove
               candle_cv_q_program_interval_list_correct;
               candle_cv_q_program_interval_matrix_correct;
               candle_cv_q_dim_taylor_upper_correct]);;
+
+let candle_cv_list_length_correct = prove
+ (`!items. candle_cv_list_length (candle_cv_q_list items) =
+           Cexp_num (LENGTH items)`,
+  LIST_INDUCT_TAC THENL
+   [REWRITE_TAC[candle_cv_q_list_def; candle_cv_list_length_def; LENGTH];
+    ASM_REWRITE_TAC[candle_cv_q_list_def; candle_cv_list_length_def;
+                    LENGTH; cexp_add_def] THEN
+    AP_TERM_TAC THEN ARITH_TAC]);;
+
+let candle_cv_instruction_lists_length_correct = prove
+ (`!programs.
+     candle_cv_list_length (candle_cv_q_instruction_lists programs) =
+     Cexp_num (LENGTH programs)`,
+  LIST_INDUCT_TAC THENL
+   [REWRITE_TAC[candle_cv_q_instruction_lists_def;
+                candle_cv_list_length_def; LENGTH];
+    ASM_REWRITE_TAC[candle_cv_q_instruction_lists_def;
+                    candle_cv_list_length_def; LENGTH; cexp_add_def;
+                    ARITH_RULE `1 + n = SUC n`]]);;
+
+let candle_cv_instruction_matrix_length_correct = prove
+ (`!program_matrix.
+     candle_cv_list_length
+       (candle_cv_q_instruction_matrix program_matrix) =
+     Cexp_num (LENGTH program_matrix)`,
+  LIST_INDUCT_TAC THENL
+   [REWRITE_TAC[candle_cv_q_instruction_matrix_def;
+                candle_cv_list_length_def; LENGTH];
+    ASM_REWRITE_TAC[candle_cv_q_instruction_matrix_def;
+                    candle_cv_list_length_def; LENGTH; cexp_add_def;
+                    ARITH_RULE `1 + n = SUC n`]]);;
+
+let candle_cv_interval_list_length_correct = prove
+ (`!boxes.
+     candle_cv_list_length (candle_cv_q_interval_list boxes) =
+     Cexp_num (LENGTH boxes)`,
+  LIST_INDUCT_TAC THENL
+   [REWRITE_TAC[candle_cv_q_interval_list_def;
+                candle_cv_list_length_def; LENGTH];
+    ASM_REWRITE_TAC[candle_cv_q_interval_list_def;
+                    candle_cv_list_length_def; LENGTH; cexp_add_def;
+                    ARITH_RULE `1 + n = SUC n`]]);;
+
+let candle_cv_q_interval_valid_correct = prove
+ (`!i.
+     candle_cv_q_le
+       (Cexp_fst (candle_cv_q_interval i))
+       (Cexp_snd (candle_cv_q_interval i)) =
+     Cexp_num (if candle_q_le (FST i) (SND i) then SUC 0 else 0)`,
+  REWRITE_TAC[candle_cv_q_interval_def; cexp_fst_def; cexp_snd_def;
+              candle_cv_q_le_correct]);;
+
+let candle_cv_q_box_valid_list_correct = prove
+ (`!boxes.
+     candle_cv_q_box_valid_list (candle_cv_q_interval_list boxes) =
+     Cexp_num (if candle_q_box_valid_list boxes then SUC 0 else 0)`,
+  LIST_INDUCT_TAC THEN
+  ASM_REWRITE_TAC[candle_cv_q_interval_list_def;
+                  candle_cv_q_box_valid_list_def;
+                  candle_q_box_valid_list_def;
+                  candle_cv_q_interval_valid_correct] THEN
+  ASM_CASES_TAC `candle_q_le (FST h) (SND h)` THEN
+  ASM_REWRITE_TAC[cexp_if_def] THEN
+  CONV_TAC NUM_REDUCE_CONV);;
+
+let candle_cv_q_rows_width_correct = prove
+ (`!n (program_matrix:((candle_q_instruction list)list)list).
+     candle_cv_q_rows_width (Cexp_num n)
+       (candle_cv_q_instruction_matrix program_matrix) =
+     Cexp_num (if candle_q_rows_width n program_matrix
+               then SUC 0 else 0)`,
+  GEN_TAC THEN LIST_INDUCT_TAC THENL
+   [REWRITE_TAC[candle_cv_q_instruction_matrix_def;
+                candle_cv_q_rows_width_def; candle_q_rows_width_def] THEN
+    CONV_TAC NUM_REDUCE_CONV;
+    ASM_REWRITE_TAC[candle_cv_q_instruction_matrix_def;
+                    candle_cv_q_rows_width_def; candle_q_rows_width_def;
+                    candle_cv_instruction_lists_length_correct;
+                    cexp_eq_def; injectivity "cval"] THEN
+    REPEAT(COND_CASES_TAC THEN ASM_REWRITE_TAC[cexp_if_def]) THEN
+    CONV_TAC NUM_REDUCE_CONV]);;
+
+let candle_cv_q_dim_inputs_valid_correct = prove
+ (`!pds pdds boxes.
+     candle_cv_q_dim_inputs_valid
+       (candle_cv_q_instruction_lists pds)
+       (candle_cv_q_instruction_matrix pdds)
+       (candle_cv_q_interval_list boxes) =
+     Cexp_num
+       (if candle_q_dim_inputs_valid pds pdds boxes
+        then SUC 0 else 0)`,
+  REPEAT GEN_TAC THEN
+  REWRITE_TAC[candle_cv_q_dim_inputs_valid_def;
+              candle_q_dim_inputs_valid_def;
+              candle_cv_instruction_lists_length_correct;
+              candle_cv_instruction_matrix_length_correct;
+              candle_cv_interval_list_length_correct;
+              candle_cv_q_rows_width_correct;
+              cexp_eq_def; injectivity "cval"] THEN
+  REPEAT(COND_CASES_TAC THEN ASM_REWRITE_TAC[cexp_if_def]) THEN
+  CONV_TAC NUM_REDUCE_CONV);;
+
+let candle_cv_q_dim_whole_box_finish_correct = prove
+ (`!inputs_valid box_valid upper.
+     candle_cv_q_dim_whole_box_finish
+       (Cexp_num (if inputs_valid then SUC 0 else 0))
+       (Cexp_num (if box_valid then SUC 0 else 0))
+       (candle_cv_q upper) =
+     Cexp_pair
+       (Cexp_num
+         (if inputs_valid /\ box_valid /\
+             ~(candle_q_le candle_q_zero upper)
+          then SUC 0 else 0))
+       (candle_cv_q upper)`,
+  REPEAT GEN_TAC THEN
+  REWRITE_TAC[candle_cv_q_dim_whole_box_finish_def;
+              candle_cv_q_zero_def; candle_cv_q_le_correct] THEN
+  ASM_CASES_TAC `inputs_valid:bool` THEN
+  ASM_CASES_TAC `box_valid:bool` THEN
+  ASM_CASES_TAC `candle_q_le candle_q_zero upper` THEN
+  ASM_REWRITE_TAC[cexp_if_def] THEN
+  CONV_TAC NUM_REDUCE_CONV);;
+
+let candle_cv_q_dim_whole_box_check_correct = prove
+ (`!pf pds pdds boxes.
+     candle_cv_q_dim_whole_box_check
+       (candle_cv_q_instruction_list pf)
+       (candle_cv_q_instruction_lists pds)
+       (candle_cv_q_instruction_matrix pdds)
+       (candle_cv_q_interval_list boxes) =
+     Cexp_pair
+       (Cexp_num
+         (if candle_q_dim_whole_box_accept pf pds pdds boxes
+          then SUC 0 else 0))
+       (candle_cv_q
+         (candle_q_dim_whole_box_upper pf pds pdds boxes))`,
+  REPEAT GEN_TAC THEN
+  REWRITE_TAC[candle_cv_q_dim_whole_box_check_def;
+              candle_cv_q_dim_inputs_valid_correct;
+              candle_cv_q_box_valid_list_correct;
+              candle_cv_q_dim_whole_box_upper_correct;
+              candle_cv_q_dim_whole_box_finish_correct;
+              candle_q_dim_whole_box_accept_def; CONJ_ASSOC]);;
 
 end;;
